papers/protocols/coq/StateMonad.v
@@ -1,0 +1,192 @@
+(*
+Definition A := Type.
+Definition S := Type.
+*)
+
+Module definition1.
+
+Definition A := nat.
+Definition S := nat.
+
+Inductive State :=
+  | state : (S -> A * S) -> State.
+
+Definition unit(x:A):State := state(fun (s:S) => (x,s)).
+
+Definition bind(m:State)(f:A -> State):State :=
+  (state (fun (s0:S) =>
+            match m with 
+              | state m' => 
+                match (m' s0) with
+                  | (a,s1) => 
+                    match (f a) with
+                      | state m'' => (m'' s1)
+                    end
+                end
+            end)).
+
+Example unit_ex1 : (unit 3) = (unit 3).
+Proof.
+  reflexivity.
+Qed.
+
+End definition1.
+
+Module definition2.
+
+Definition A := nat.
+Definition S := nat.
+
+Definition State := S -> A * S.
+
+Definition unit(x:A):State := (fun (s:S) => (x,s)).
+
+Definition bind(m:State)(f:A -> State):State :=
+  (fun (s0:S) =>
+     match (m s0) with
+           | (a,s1) => (f a) s1
+     end).
+
+Definition sequence(m:State)(n:State):State :=
+  (fun (s0:S) =>
+     match (m s0) with
+           | (a,s1) => n s1
+     end).
+
+Example unit_ex1 : unit(0)(1) = (0,1).
+Proof.
+  unfold unit.
+  reflexivity.
+Qed.
+
+Example bind_ex1 : ((bind (unit 0) (fun (a:A) => (fun (s:S) => (a,(s+1))))) 0) = (0,1).
+Proof.
+  unfold bind. reflexivity.
+Qed.
+
+Example bind_ex2 : ((bind
+                       (bind
+                          (unit 0) (fun (a:A) => (fun (s:S) => (0,(s+1)))))
+                       (fun (a:A) => (fun (s:S) => (0,(s+1))))) 0) = (0,2).
+Proof.
+  unfold bind. reflexivity.
+Qed.
+
+Notation "m >>= f" :=
+  (bind m f) (left associativity, at level 49).
+
+Notation "m >> f" :=
+  (sequence m f) (left associativity, at level 49).
+
+Example bind_ex1' : ((unit 0) >>= (fun (a:A) => (fun (s:S) => (a,(s+1))))) 0 = (0,1).
+Proof.
+  unfold bind. reflexivity.
+Qed.
+
+Example bind_ex2' : (((unit 0) >>= (fun (a:A) => (fun (s:S) => (0,(s+1)))))
+                               >>= (fun (a:A) => (fun (s:S) => (0,(s+1))))) 0
+                    = (0,2).
+Proof.
+  unfold bind. reflexivity.
+Qed.
+
+(* Not at all this notation is useful given that it appears to sequence only
+   two operations and does not support sequence. *)
+
+Notation "'do' a <- e ; c" :=
+  (e >>= (fun a => c)) (at level 59, right associativity).
+
+Example bind_ex1'' : (do a <- (unit 0) ; (fun (s:S) => (0,(s+1)))) 0 = (0,1).
+Proof.
+  unfold bind. reflexivity.
+Qed.
+
+End definition2.
+
+Module definition3.
+
+(* Let's parameterize State over types *)
+
+Definition State (S A:Type) := S -> A * S.
+
+Definition unit{S A:Type}(x:A):(State S A) := (fun (s:S) => (x,s)).
+
+Definition bind{S A:Type}(m:(State S A))(f:A -> (State S A)):(State S A) :=
+  (fun (s0:S) =>
+     match (m s0) with
+           | (a,s1) => (f a) s1
+     end).
+
+Definition sequence{S A:Type}(m:(State S A))(n:(State S A)):(State S A) :=
+  (fun (s0:S) =>
+     match (m s0) with
+           | (a,s1) => n s1
+     end).
+
+Example unit_ex1 : unit(0)(1) = (0,1).
+Proof.
+  unfold unit.
+  reflexivity.
+Qed.
+
+Example bind_ex1: ((bind (unit 0) (fun a => (fun s => (a,(s+1))))) 0) = (0,1).
+Proof.
+  unfold bind. reflexivity.
+Qed.
+
+Example bind_ex2 : ((bind
+                       (bind
+                          (unit 0) (fun a => (fun s => (0,(s+1)))))
+                       (fun a => (fun s => (0,(s+1))))) 0) = (0,2).
+Proof.
+  unfold bind. reflexivity.
+Qed.
+
+End definition3.
+
+Module definition4.
+
+(* Let's make this puppy a monad using a typeclass *)
+
+Class Monad (M: Type -> Type):Type := 
+{
+  unit: forall {A}, A -> M A
+  ; bind: forall {A B}, M A -> (A -> (M B)) -> M B
+  ; left_unit : forall {A B} (a:A) (f:A -> M B), bind (unit a) f = f a
+  ; right_unit : forall {A} (ma:M A), bind ma unit = ma
+  ; assoc : forall {A B C} (ma:M A) (f:A -> M B) (g:B -> M C),
+              bind (bind ma f) g = bind ma (fun a => bind (f a) g)
+}.
+
+Definition State (S A:Type) := S -> A * S.
+
+Instance StateMonad : Monad (State nat) :=
+{
+  unit A x := (fun s => (x,s))
+  ; bind S A m f := (fun s0 =>
+                       match (m s0) with
+                         | (a,s1) => (f a) s1
+                       end)
+}.
+Proof.
+  intros. reflexivity.
+Admitted.
+
+Example unit_ex1 : unit(0)(1) = (0,1).
+Proof.
+  unfold unit.
+  reflexivity.
+Qed.
+
+Example bind_ex1: ((bind (unit 0) (fun a => (fun s => (a,(s+1))))) 0) = (0,1).
+Proof.
+  unfold bind. reflexivity.
+Qed.
+
+Example bind_ex2 : ((bind
+                       (bind
+                          (unit 0) (fun a => (fun s => (0,(s+1)))))
+                       (fun a => (fun s => (0,(s+1))))) 0) = (0,2).
+Proof.
+  unfold bind. reflexivity.
+Qed.
